sketch "stateless" (trace-inspecting) e1000_step directly in wp
and discovered in the spec that reading RDH to determine which
buffers are finished is not reliable, nor is reading TDH to
determine which buffers can be returned to the memory pool.
So we'd need to check the DD (descriptor-done) status bit instead,
so software needs to read memory that gets written concurrently
by hardware, so we can't assign clear unique ownership to each
memory chunk...

bedrock2/src/bedrock2/TraceInspection.v
@@ -1,9 +1,20 @@
 Require Import Coq.Strings.String.
 Require Import Coq.ZArith.ZArith.
+Require Import coqutil.Tactics.Tactics.
 Require Import coqutil.Tactics.fwd.
 Require Import coqutil.Map.Interface coqutil.Map.Properties.
 Require Import coqutil.Word.Interface coqutil.Word.Bitwidth.
 Require Import bedrock2.Syntax bedrock2.Semantics.
+
+Record RegisterSpec{width: Z}{BW: Bitwidth width}{word: word.word width} := {
+  initial_register_value: option word;
+  register_address: word;
+}.
+
+Record RegisterBehavior{width: Z}{BW: Bitwidth width}{word: word.word width} := {
+  read: Prop;
+  write: word -> Prop;
+}.
 
 Section WithMem.
   Context {width: Z} {BW: Bitwidth width}
@@ -29,18 +40,29 @@ Section WithMem.
       end
     else None.
 
-  Fixpoint get_rw_reg(t: trace)(addr: word): option word :=
+  Definition InitializedRegister(addr initial: Z): RegisterSpec := {|
+    initial_register_value := Some (word.of_Z initial);
+    register_address := word.of_Z addr;
+  |}.
+
+  Definition UninitializedRegister(addr: Z): RegisterSpec := {|
+    initial_register_value := None;
+    register_address := word.of_Z addr;
+  |}.
+
+
+  Fixpoint get_rw_reg0(t: trace)(addr: word): option word :=
     match t with
     | nil => None
     | cons e rest =>
         match get_rw_reg_in_event e addr with
         | Some v => Some v
-        | None => get_rw_reg rest addr
+        | None => get_rw_reg0 rest addr
         end
     end.
 
   (* the same definition with a more separation-logic-like signature: *)
-  Definition rw_reg(val addr: word): trace -> Prop :=
+  Definition uninitialized_rw_reg(val addr: word): trace -> Prop :=
     fix rec t :=
       match t with
       | nil => False
@@ -51,11 +73,78 @@ Section WithMem.
           end
       end.
 
+  Definition initialized_rw_reg(initial val addr: word): trace -> Prop :=
+    fix rec t :=
+      match t with
+      | nil => initial = val
+      | cons e tail =>
+          match get_rw_reg_in_event e addr with
+          | Some v => v = val
+          | None => rec tail
+          end
+      end.
+
+  Definition rw_reg(r: RegisterSpec)(val: word): trace -> Prop :=
+    fix rec t :=
+      match t with
+      | nil => initial_register_value r = Some val
+      | cons e tail =>
+          match get_rw_reg_in_event e (register_address r) with
+          | Some v => v = val
+          | None => rec tail
+          end
+      end.
+
+  Context {word_ok: word.ok word} {mem_ok: map.ok mem}.
+
+  Lemma uninitialized_rw_reg_unique: forall t addr val1 val2,
+      uninitialized_rw_reg val1 addr t ->
+      uninitialized_rw_reg val2 addr t ->
+      val1 = val2.
+  Proof.
+    induction t; simpl; intros.
+    - contradiction.
+    - destruct_one_match_hyp. 1: congruence. eauto.
+  Qed.
+
+  Lemma initialized_rw_reg_unique: forall t addr init val1 val2,
+      initialized_rw_reg init val1 addr t ->
+      initialized_rw_reg init val2 addr t ->
+      val1 = val2.
+  Proof.
+    induction t; simpl; intros.
+    - congruence.
+    - destruct_one_match_hyp. 1: congruence. eauto.
+  Qed.
+
+  Lemma rw_reg_unique: forall r t val1 val2,
+      rw_reg r val1 t ->
+      rw_reg r val2 t ->
+      val1 = val2.
+  Proof.
+    destruct r as (init & addr).
+    induction t; simpl; intros.
+    - congruence.
+    - destruct_one_match_hyp. 1: congruence. eauto.
+  Qed.
+
+  Definition get_rw_reg(r: RegisterSpec)(t: trace)(k: word -> Prop): Prop :=
+    exists val, rw_reg r val t /\ k val.
+
   (* TODO can we define separating conjunction on (trace -> Prop)? *)
 
-  (* TODO clear-on-write semantics etc? *)
   (* TODO getters for different write semantics and different initial values,
-     then define get_E1000_MYREGNAME using one of these getters --> looks like section 13 *)
+     then define get_E1000_MYREG using one of these getters --> looks like section 13 *)
+
+  (* Interesting registers:
+     13.4.17 Interrupt Cause Read Register ICR: read-only, clear-on-read,
+     but writing also allowed, writing 1 clears bit, writing 0 has no effect.
+     13.4.19 Interrupt Cause Set Register ICS: write-only,
+     writing 1 sets bit in ICR, writing 0 has no effect.
+     13.4.20 Interrupt Mask Set/Read Register IMS: read-write,
+     writing 1 sets bit, writing 0 has no effect, reading returns all enabled bits.
+     13.4.21 Interrupt Mask Clear Register IMC: write-only,
+     writing 1 clears bit in IMS, writing 0 has no effect *)
 
   (* (externally_owned_mem t m) means that after trace t has happened, the memory
      owned by the external world (i.e the memory that was given away by software
@@ -68,4 +157,37 @@ Section WithMem.
                        exists mKeep, map.split m_prev mKeep mGive /\
                                      map.split m mKeep mReceive
     end.
+
+  Lemma externally_owned_mem_unique: forall t m1 m2,
+      externally_owned_mem t m1 ->
+      externally_owned_mem t m2 ->
+      m1 = m2.
+  Proof.
+    induction t; simpl; intros.
+    - subst. reflexivity.
+    - destruct a as (((mGive & action) & args) & (mReceive & rets)). fwd.
+      specialize IHt with (1 := H0p0) (2 := Hp0). subst m_prev0.
+      pose proof (proj1 (map.split_diff (map.same_domain_refl _) Hp1p0 H0p1p0)).
+      subst mKeep0.
+      apply proj1 in Hp1p1. apply proj1 in H0p1p1. subst m1 m2. reflexivity.
+  Qed.
+
+  Definition dispatch(action: String.string)(args: list word):
+    list (RegisterSpec * RegisterBehavior) -> Prop :=
+    fix rec bs :=
+      match bs with
+      | nil => False
+      | cons (r, b) tail =>
+          match args with
+          | cons addr args' =>
+              if word.eqb (register_address r) addr then
+                match args' with
+                | nil => action = "MMIOREAD"%string /\ b.(read)
+                | cons val nil => action = "MMIOWRITE"%string /\ b.(write) val
+                | _ => False
+                end
+              else rec tail
+          | _ => False
+          end
+      end.
 End WithMem.
